proof of Scheme semantics progress, adjusted begin expression semantics, no build

compiler/scheme/scheme_astScript.sml
@@ -24,7 +24,7 @@ Datatype:
       | Cond exp exp exp
       | Ident mlstring
       | Lambda (mlstring list) (mlstring option) exp
-      | Begin exp (exp list)
+      | Begin (exp list) exp
       | Set mlstring exp
       | Letrec ((mlstring # exp) list) exp
 End
@@ -33,7 +33,7 @@ Datatype:
   (*Contexts for small-step operational semantics*)
   cont = ApplyK ((val # val list) option) (exp list)
        | CondK exp exp
-       | BeginK (exp list)
+       | BeginK (exp list) exp
        | SetK mlstring
 ;
   val = Prim prim | SNum int | Wrong string | SBool bool
@@ -49,38 +49,91 @@ Definition lit_to_val_def:
   lit_to_val (LitBool b) = SBool b
 End
 
-Definition static_scoping_check_def:
-  (static_scoping_check env (Cond c t f) ⇔
-    static_scoping_check env c ∧
-    static_scoping_check env t ∧
-    static_scoping_check env f) ∧
-  (static_scoping_check env (Apply e args) ⇔
-    static_scoping_check env e ∧
-    EVERY (static_scoping_check env) args) ∧
-  (static_scoping_check env (Set _ e) ⇔ static_scoping_check env e) ∧
-  (static_scoping_check env (Begin e es) ⇔
-    static_scoping_check env e ∧
-    EVERY (static_scoping_check env) es) ∧
-  (static_scoping_check env (Lambda xs xp e) ⇔ let xs' = case xp of
-    | NONE => xs
-    | SOME x => x::xs
-    in ALL_DISTINCT xs' ∧ static_scoping_check (env ∪ set xs') e) ∧
-  (static_scoping_check env (Letrec xes e) ⇔ let xs = MAP FST xes
-    in ALL_DISTINCT xs ∧ let env' = env ∪ set xs
-    in static_scoping_check env' e ∧
-       EVERY (static_scoping_check env') (MAP SND xes)) ∧
-  (static_scoping_check env (Ident x) ⇔ env x) ∧
-  (static_scoping_check _ _ ⇔ T)
-Termination
-  WF_REL_TAC ‘measure $ exp_size o SND’
-  >> Induct_on ‘xes’ >- (rw[])
-  >> Cases_on ‘h’
-  >> simp[snd (TypeBase.size_of “:exp”), list_size_def, snd (TypeBase.size_of “:'a # 'b”)]
-  >> rpt strip_tac >- (rw[])
-  >> last_x_assum $ qspecl_then [‘e’, ‘a’] $ imp_res_tac
-  >> first_x_assum $ qspec_then ‘e’ $ assume_tac
-  >> rw[]
+Inductive static_scope:
+[~Lit:]
+  static_scope env (Lit lit)
+[~Cond:]
+  static_scope env c ∧
+  static_scope env t ∧
+  static_scope env f
+  ⇒
+  static_scope env (Cond c t f)
+[~Apply:]
+  static_scope env fn ∧
+  EVERY (static_scope env) es
+  ⇒
+  static_scope env (Apply fn es)
+[~Begin:]
+  EVERY (static_scope env) es ∧
+  static_scope env e
+  ⇒
+  static_scope env (Begin es e)
+[~Lambda_NONE:]
+  ALL_DISTINCT xs ∧
+  static_scope (env ∪ set xs) e
+  ⇒
+  static_scope env (Lambda xs NONE e)
+[~Lambda_SOME:]
+  ALL_DISTINCT (x::xs) ∧
+  static_scope (env ∪ set (x::xs)) e
+  ⇒
+  static_scope env (Lambda xs (SOME x) e)
+[~Letrec:]
+  ALL_DISTINCT (MAP FST bs) ∧
+  EVERY (static_scope (env ∪ set (MAP FST bs))) (MAP SND bs) ∧
+  static_scope (env ∪ set (MAP FST bs)) e
+  ⇒
+  static_scope env (Letrec bs e)
+[~Ident:]
+  env x
+  ⇒
+  static_scope env (Ident x)
+[~Set:]
+  env x ∧
+  static_scope env e
+  ⇒
+  static_scope env (Set x e)
 End
+
+Definition exp_rec_def:
+  exp_rec (Lit l) = 1 ∧
+  exp_rec (Cond c t f) = exp_rec c + exp_rec t + exp_rec f ∧
+  exp_rec (Apply fn es) = exp_rec fn + SUM (MAP exp_rec es) ∧
+  exp_rec (Begin es e) = exp_rec e + SUM (MAP exp_rec es) ∧
+  exp_rec (Lambda xs xp e) = exp_rec e ∧
+  exp_rec (Letrec bs e) = exp_rec e + SUM (MAP (exp_rec o SND) bs)∧
+  exp_rec (Ident x) = 1 ∧
+  exp_rec (Set x e) =  exp_rec e
+Termination
+  WF_REL_TAC ‘measure exp_size’
+End
+
+Theorem static_scope_mono:
+  ∀ env e env' .
+    env ⊆ env' ∧ static_scope env e ⇒ static_scope env' e
+Proof
+  simp[Once CONJ_COMM]
+  >> simp[GSYM AND_IMP_INTRO]
+  >> simp[GSYM PULL_FORALL]
+  >> ho_match_mp_tac static_scope_ind
+  >> rpt strip_tac
+  >~ [‘Letrec bs e’] >- (
+    simp[Once static_scope_cases]
+    >> ‘env ∪ set (MAP FST bs) ⊆ env' ∪ set (MAP FST bs)’
+      by gvs[SUBSET_UNION_ABSORPTION, UNION_ASSOC]
+    >> qpat_x_assum ‘∀ _._ ⇒ _’ $ irule_at (Pos last)
+    >> simp[]
+    >> irule EVERY_MONOTONIC
+    >> qpat_x_assum ‘EVERY _ _’ $ irule_at (Pos last)
+    >> rpt strip_tac
+    >> gvs[]
+  )
+  >> simp[Once static_scope_cases]
+  >> gvs[SUBSET_DEF, SPECIFICATION]
+  >> irule EVERY_MONOTONIC
+  >> qpat_assum ‘EVERY _ _’ $ irule_at (Pos last)
+  >> gvs[]
+QED
 
 val _ = export_theory();
 
