compiler/scheme/scheme_semanticsScript.sml
@@ -56,12 +56,12 @@ Definition fresh_loc_def:
 End
 
 Definition parameterize_def:
-  parameterize store ks env [] NONE e [] = (store, ks, env, Exp e) ∧
-  parameterize store ks env [] (SOME (l:mlstring)) e xs = (let (n, store') = fresh_loc store (SOME $ SList xs)
-    in (store', ks, (env |+ (l, n)), Exp e)) ∧
-  parameterize store ks env (p::ps) lp e (x::xs) = (let (n, store') = fresh_loc store (SOME x)
-    in parameterize store' ks (env |+ (p, n)) ps lp e xs) ∧
-  parameterize store ks _ _ _ _ _ = (store, ks, FEMPTY, Exception $ strlit "Wrong number of arguments")
+  parameterize store env [] NONE e [] = (store, env, Exp e) ∧
+  parameterize store env [] (SOME (l:mlstring)) e xs = (let (n, store') = fresh_loc store (SOME $ SList xs)
+    in (store', (env |+ (l, n)), Exp e)) ∧
+  parameterize store env (p::ps) lp e (x::xs) = (let (n, store') = fresh_loc store (SOME x)
+    in parameterize store' (env |+ (p, n)) ps lp e xs) ∧
+  parameterize store _ _ _ _ _ = (store, FEMPTY, Exception $ strlit "Wrong number of arguments")
 End
 
 Definition application_def:
@@ -73,8 +73,8 @@ Definition application_def:
   | CallCC => case xs of
     | [v] => (store, (FEMPTY, ApplyK (SOME (v, [])) []) :: ks, FEMPTY, Val $ Throw ks)
     | _ => (store, ks, FEMPTY, Exception $ strlit "Arity mismatch")) ∧
-  application store ks (Proc env ps lp e) xs =
-    parameterize store ks env ps lp e xs ∧
+  application store ks (Proc env ps lp e) xs = (let (store', env', e') =
+    parameterize store env ps lp e xs in (store', ks, env', e')) ∧
   application store ks (Throw ks') xs = (case xs of
     | [v] => (store, ks', FEMPTY, Val v)
     | _ => (store, ks, FEMPTY, Exception $ strlit "Arity mismatch")) ∧
@@ -94,9 +94,9 @@ Definition return_def:
   return store ((env, CondK t f) :: ks) v = (if v = (SBool F)
     then (store, ks, env, Exp f) else (store, ks, env, Exp t)) ∧
 
-  return store ((env, BeginK es) :: ks) v = (case es of
-  | [] => (store, ks, env, Val v)
-  | e::es' => (store, (env, BeginK es') :: ks, env, Exp e)) ∧
+  return store ((env, BeginK es e) :: ks) v = (case es of
+  | [] => (store, ks, env, Exp e)
+  | e'::es' => (store, (env, BeginK es' e) :: ks, env, Exp e')) ∧
   return store ((env, SetK x) :: ks) v = (LUPDATE (SOME v) (env ' x) store, ks, env, Val $ Wrong "Unspecified")
 End
 
@@ -117,13 +117,14 @@ Definition step_def:
     | SOME v => Val v
     in (store, ks, env, ev)) ∧
   step (store, ks, env, Exp $ Lambda ps lp e) = (store, ks, env, Val $ Proc env ps lp e) ∧
-  step (store, ks, env, Exp $ Begin e es) = (store, (env, BeginK es) :: ks, env, Exp e) ∧
+  step (store, ks, env, Exp $ Begin es e) = (case es of
+  | [] => (store, ks, env, Exp e)
+  | e'::es' => (store, (env, BeginK es' e) :: ks, env, Exp e')) ∧
   step (store, ks, env, Exp $ Set x e) = (store, (env, SetK x) :: ks, env, Exp e) ∧
   (*There is a missing reinit check, though the spec says it is optional*)
-  step (store, ks, env, Exp $ Letrec bs e) = (case bs of
-  | [] => (store, ks, env, Exp e)
-  | (x, i)::bs' => let (store', env') = letrec_init store env (MAP FST bs)
-      in (store', (env', BeginK (SNOC e (MAP (UNCURRY Set) bs'))) :: ks, env', Exp $ Set x i)) ∧
+  step (store, ks, env, Exp $ Letrec bs e) = (let
+    (store', env') = letrec_init store env (MAP FST bs)
+      in (store', ks, env', Exp $ Begin (MAP (UNCURRY Set) bs) e)) ∧
 
   step (store, ks, env, Exception ex) = (store, [], env, Exception ex)
 End
@@ -132,6 +133,874 @@ Definition steps_def:
   steps (n:num) t = if n = 0 then t
     else steps (n - 1) $ step t
 End
+
+Definition option_to_set_def:
+  option_to_set NONE = ∅ ∧
+  option_to_set (SOME x) = {x}
+End
+
+Inductive can_lookup:
+  FEVERY (λ (x, n). n < LENGTH store) env
+  ⇒
+  can_lookup env store
+End
+
+Inductive valid_val:
+[~val_SNum:]
+  valid_val store (SNum n)
+[~val_SBool:]
+  valid_val store (SBool b)
+[~val_Prim:]
+  valid_val store (Prim p)
+[~val_Wrong:]
+  valid_val store (Wrong w)
+[~val_SList:]
+  EVERY (valid_val store) vs
+  ⇒
+  valid_val store (SList vs)
+[~val_Proc_NONE:]
+  static_scope (FDOM env ∪ set xs) e ∧
+  can_lookup env store
+  ⇒
+  valid_val store (Proc env xs NONE e)
+[~val_Proc_SOME:]
+  static_scope (FDOM env ∪ set (x::xs)) e ∧
+  can_lookup env store
+  ⇒
+  valid_val store (Proc env xs (SOME x) e)
+[~val_Throw:]
+  valid_cont store ks
+  ⇒
+  valid_val store (Throw ks)
+
+[~cont_Id:]
+  valid_cont store []
+[~cont_CondK:]
+  static_scope (FDOM env) t ∧
+  static_scope (FDOM env) f ∧
+  valid_cont store ks ∧
+  can_lookup env store
+  ⇒
+  valid_cont store ((env, CondK t f)::ks)
+[~cont_ApplyK_NONE:]
+  EVERY (static_scope (FDOM env)) es ∧
+  valid_cont store ks ∧
+  can_lookup env store
+  ⇒
+  valid_cont store ((env, ApplyK NONE es)::ks)
+[~cont_ApplyK_SOME:]
+  valid_val store fn ∧
+  EVERY (valid_val store) vs ∧
+  EVERY (static_scope (FDOM env)) es ∧
+  valid_cont store ks ∧
+  can_lookup env store
+  ⇒
+  valid_cont store ((env, ApplyK (SOME (fn, vs)) es)::ks)
+[~cont_BeginK:]
+  EVERY (static_scope (FDOM env)) es ∧
+  static_scope (FDOM env) e ∧
+  valid_cont store ks ∧
+  can_lookup env store
+  ⇒
+  valid_cont store ((env, BeginK es e)::ks)
+[~cont_SetK:]
+  (FDOM env) x ∧
+  valid_cont store ks ∧
+  can_lookup env store
+  ⇒
+  valid_cont store ((env, SetK x)::ks)
+End
+
+Inductive valid_state:
+[~Val:]
+  valid_val store v ∧
+  valid_cont store ks ∧
+  can_lookup env store ∧
+  EVERY (OPTION_ALL (valid_val store)) store
+  ⇒
+  valid_state store ks env (Val v)
+[~Exp:]
+  static_scope (FDOM env) e ∧
+  valid_cont store ks ∧
+  can_lookup env store ∧
+  EVERY (OPTION_ALL (valid_val store)) store
+  ⇒
+  valid_state store ks env (Exp e)
+[~Exception:]
+  valid_state store ks env (Exception s)
+End
+
+Theorem FEVERY_MONO:
+  ∀ P Q f .
+    (∀ x . P x ⇒ Q x) ∧ FEVERY P f
+    ⇒
+    FEVERY Q f
+Proof
+  Induct_on ‘f’
+  >> rpt strip_tac >- simp[FEVERY_FEMPTY]
+  >> last_x_assum $ drule_then assume_tac
+  >> gvs[FEVERY_FUPDATE]
+  >> qsuff_tac ‘DRESTRICT f (COMPL {x}) = f’ >- (strip_tac >> gvs[])
+  >> simp[EQ_FDOM_SUBMAP, DRESTRICT_DEF, EXTENSION]
+  >> strip_tac
+  >> iff_tac
+  >> rpt strip_tac
+  >> gvs[]
+QED
+
+Theorem EVERY_OPTION_ALL_MAP_SOME:
+  ∀ f xs . EVERY f xs ⇒ EVERY (OPTION_ALL f) (MAP SOME xs)
+Proof
+  strip_tac
+  >> Induct
+  >> simp[]
+QED
+
+Theorem EVERY_TAKE:
+  ∀ f n xs . EVERY f xs ⇒ EVERY f (TAKE n xs)
+Proof
+  gen_tac
+  >> Induct_on ‘xs’
+  >> Cases_on ‘n’
+  >> simp[]
+QED
+
+Theorem valid_larger_store:
+  ∀ (store :'a list) (store' :'a list) .
+    LENGTH store ≤ LENGTH store'
+    ⇒
+    (∀ v .
+      valid_val store v
+      ⇒
+      valid_val store' v) ∧
+    ∀ ks .
+      valid_cont store ks
+      ⇒
+      valid_cont store' ks
+Proof
+  rpt gen_tac >> strip_tac
+  >> ho_match_mp_tac valid_val_ind
+  >> rpt strip_tac
+  >> simp[Once valid_val_cases]
+  >> gvs[can_lookup_cases]
+  >> gvs[SF ETA_ss]
+  >> irule FEVERY_MONO
+  >> pop_assum $ irule_at (Pos last)
+  >> PairCases
+  >> rpt strip_tac
+  >> gvs[]
+QED
+
+Theorem valid_val_larger_store = SRULE [PULL_FORALL, AND_IMP_INTRO] $
+  cj 1 valid_larger_store;
+Theorem valid_cont_larger_store = SRULE [PULL_FORALL, AND_IMP_INTRO] $
+  cj 2 valid_larger_store;
+
+Theorem letrec_init_mono:
+  ∀ bs store env store' env' .
+    letrec_init store env bs = (store', env')
+    ⇒
+    FDOM env ⊆ FDOM env'
+Proof
+  Induct
+  >> simp[letrec_init_def]
+  >> rpt strip_tac
+  >> rpt (pairarg_tac >> gvs[])
+  >> last_x_assum drule
+  >> simp[]
+QED
+
+Theorem letrec_init_dom:
+  ∀ xs store env store' env' .
+    letrec_init store env xs = (store', env')
+    ⇒
+    FDOM env ∪ set xs = FDOM env' ∧
+    store ++ GENLIST (λ x. NONE) (LENGTH xs) = store'
+Proof
+  Induct
+  >> simp[letrec_init_def, fresh_loc_def]
+  >> rpt strip_tac
+  >> rpt (pairarg_tac >> gvs[])
+  >> last_x_assum $ drule_then assume_tac
+  >> gvs[GENLIST] >- (
+    rpt strip_tac
+    >> qpat_x_assum ‘_ ∪ _ = _’ $ simp o single o GSYM
+    >> simp[EXTENSION]
+    >> simp[UNION_DEF, INSERT_DEF, SPECIFICATION, GSYM DISJ_ASSOC]
+    >> strip_tac
+    >> iff_tac
+    >> rw[] >> rw[]
+  )
+  >> rpt $ pop_assum kall_tac
+  >> ‘∃ n . LENGTH xs = n’ by simp[]
+  >> simp[]
+  >> pop_assum kall_tac
+  >> Induct_on ‘n’
+  >> simp[GENLIST]
+QED
+
+Theorem letrec_init_lookup:
+  ∀ xs store env store' env' .
+    can_lookup env store ∧
+    letrec_init store env xs = (store', env')
+    ⇒
+    can_lookup env' store'
+Proof
+  Induct
+  >> simp[letrec_init_def, fresh_loc_def]
+  >> rpt strip_tac
+  >> rpt (pairarg_tac >> gvs[])
+  >> qsuff_tac ‘can_lookup (env |+ (h,LENGTH store)) (SNOC NONE store)’ >- (
+    strip_tac
+    >> last_x_assum drule_all
+    >> simp[]
+  )
+  >> gvs[can_lookup_cases]
+  >> qsuff_tac ‘FEVERY (λ(x,n). n < SUC (LENGTH store)) env’ >- (
+    strip_tac
+    >> irule $ cj 2 FEVERY_STRENGTHEN_THM
+    >> simp[]
+  )
+  >> irule FEVERY_MONO
+  >> qpat_assum ‘FEVERY _ _’ $ irule_at (Pos last)
+  >> PairCases
+  >> simp[]
+QED
+
+Theorem parameterize_NONE_dom:
+  ∀ xs store env vs store' env' e e' .
+    LENGTH xs = LENGTH vs ∧
+    parameterize store env xs NONE e vs = (store', env', e')
+    ⇒
+    Exp e = e' ∧
+    FDOM env ∪ set xs = FDOM env' ∧
+    store ++ MAP SOME vs = store'
+Proof
+  Induct
+  >> simp[parameterize_def]
+  >> Cases_on ‘vs’
+  >> simp[parameterize_def]
+  >> rpt strip_tac
+  >> rpt (pairarg_tac >> gvs[])
+  >> last_x_assum $ drule_at (Pos $ el 2)
+  >> rpt strip_tac
+  >> gvs[] >- (
+    pop_assum $ simp o single o GSYM
+    >> simp[Once INSERT_SING_UNION, EXTENSION]
+    >> strip_tac
+    >> iff_tac
+    >> strip_tac
+    >> simp[]
+  )
+  >> gvs[fresh_loc_def]
+QED
+
+Theorem parameterize_NONE_lookup:
+  ∀ xs store env vs store' env' e e' .
+    LENGTH xs = LENGTH vs ∧
+    can_lookup env store ∧
+    parameterize store env xs NONE e vs = (store', env', e')
+    ⇒
+    can_lookup env' store'
+Proof
+  Induct
+  >> simp[parameterize_def]
+  >> Cases_on ‘vs’
+  >> simp[parameterize_def]
+  >> rpt strip_tac
+  >> rpt (pairarg_tac >> gvs[])
+  >> last_x_assum $ drule_at (Pos $ el 3)
+  >> rpt strip_tac
+  >> gvs[]
+  >> pop_assum irule
+  >> gvs[can_lookup_cases, fresh_loc_def]
+  >> irule $ cj 2 FEVERY_STRENGTHEN_THM
+  >> simp[]
+  >> irule $ FEVERY_MONO
+  >> qpat_assum ‘FEVERY _ _’ $ irule_at (Pos last)
+  >> PairCases
+  >> simp[]
+QED
+
+Theorem parameterize_NONE_exception:
+  ∀ xs store env vs store' env' e e' .
+    LENGTH xs ≠ LENGTH vs ∧
+    parameterize store env xs NONE e vs = (store', env', e')
+    ⇒
+    ∃ s . Exception s = e'
+Proof
+  Induct
+  >> Cases_on ‘vs’
+  >> simp[parameterize_def]
+  >> rpt strip_tac
+  >> rpt (pairarg_tac >> gvs[])
+  >> last_x_assum drule_all
+  >> simp[]
+QED
+
+Theorem parameterize_SOME_dom:
+  ∀ xs vs store env x store' env' e e' .
+    LENGTH xs ≤ LENGTH vs ∧
+    parameterize store env xs (SOME x) e vs = (store', env', e')
+    ⇒
+    Exp e = e' ∧
+    FDOM env ∪ set (x::xs) = FDOM env' ∧
+    store ++ MAP SOME (TAKE (LENGTH xs) vs)
+      ++ [SOME (SList (REVERSE (TAKE (LENGTH vs - LENGTH xs) (REVERSE vs))))]
+      = store'
+Proof
+  gen_tac >> gen_tac
+  >> ‘∃ n . n = LENGTH vs - LENGTH xs’ by simp[]
+  >> pop_assum mp_tac
+  >> qid_spec_tac ‘vs’
+  >> Induct_on ‘xs’
+  >> simp[parameterize_def, fresh_loc_def] >- (
+    strip_tac >> strip_tac
+    >> simp_tac bool_ss [Once $ GSYM LENGTH_REVERSE]
+    >> simp[TAKE_LENGTH_ID]
+    >> simp[Once UNION_COMM]
+    >> simp[Once $ GSYM INSERT_SING_UNION]
+  )
+  >> Cases_on ‘vs’
+  >> simp[parameterize_def]
+  >> rpt strip_tac
+  >> rpt (pairarg_tac >> gvs[])
+  >> last_x_assum $ drule_at (Pos $ el 3)
+  >> rpt strip_tac
+  >> gvs[fresh_loc_def] >- (
+    pop_assum $ simp o single o GSYM
+    >> simp[EXTENSION]
+    >> strip_tac
+    >> iff_tac
+    >> strip_tac
+    >> simp[]
+  )
+  >> simp[TAKE_APPEND1]
+QED
+
+Theorem parameterize_SOME_lookup:
+  ∀ xs vs store env x store' env' e e' .
+    LENGTH xs ≤ LENGTH vs ∧
+    can_lookup env store ∧
+    parameterize store env xs (SOME x) e vs = (store', env', e')
+    ⇒
+    can_lookup env' store'
+Proof
+  gen_tac >> gen_tac
+  >> ‘∃ n . n = LENGTH vs - LENGTH xs’ by simp[]
+  >> pop_assum mp_tac
+  >> qid_spec_tac ‘vs’
+  >> Induct_on ‘xs’
+  >> simp[parameterize_def, fresh_loc_def] >- (
+    simp[can_lookup_cases]
+    >> rpt strip_tac
+    >> irule $ cj 2 FEVERY_STRENGTHEN_THM
+    >> simp[]
+    >> irule $ FEVERY_MONO
+    >> qpat_assum ‘FEVERY _ _’ $ irule_at (Pos last)
+    >> PairCases
+    >> simp[]
+  )
+  >> Cases_on ‘vs’
+  >> simp[parameterize_def]
+  >> rpt strip_tac
+  >> rpt (pairarg_tac >> gvs[])
+  >> last_x_assum $ drule_at (Pos $ el 4)
+  >> rpt strip_tac
+  >> gvs[]
+  >> pop_assum irule
+  >> gvs[fresh_loc_def, can_lookup_cases]
+  >> irule $ cj 2 FEVERY_STRENGTHEN_THM
+  >> simp[]
+  >> irule $ FEVERY_MONO
+  >> qpat_assum ‘FEVERY _ _’ $ irule_at (Pos last)
+  >> PairCases
+  >> simp[]
+QED
+
+Theorem parameterize_SOME_exception:
+  ∀ xs store env x vs store' env' e e' .
+    LENGTH vs < LENGTH xs ∧
+    parameterize store env xs (SOME x) e vs = (store', env', e')
+    ⇒
+    ∃ s . Exception s = e'
+Proof
+  Induct
+  >> Cases_on ‘vs’
+  >> simp[parameterize_def]
+  >> rpt strip_tac
+  >> rpt (pairarg_tac >> gvs[])
+  >> last_x_assum drule_all
+  >> simp[]
+QED
+
+Theorem sadd_num_or_exception:
+  ∀ vs n .
+    (∃ m . sadd vs n = Val (SNum m)) ∨
+    (∃ s . sadd vs n = Exception s)
+Proof
+  Induct
+  >> simp[sadd_def]
+  >> Cases
+  >> simp[sadd_def]
+QED
+
+Theorem smul_num_or_exception:
+  ∀ vs n .
+    (∃ m . smul vs n = Val (SNum m)) ∨
+    (∃ s . smul vs n = Exception s)
+Proof
+  Induct
+  >> simp[smul_def]
+  >> Cases
+  >> simp[smul_def]
+QED
+
+Theorem sminus_num_or_exception:
+  ∀ vs .
+    (∃ m . sminus vs = Val (SNum m)) ∨
+    (∃ s . sminus vs = Exception s)
+Proof
+  Cases
+  >> simp[sminus_def]
+  >> Cases_on ‘h’
+  >> simp[sminus_def]
+  >> qspecl_then [‘t’, ‘0’] assume_tac sadd_num_or_exception
+  >> EVERY_CASE_TAC
+  >> gvs[]
+QED
+
+Theorem seqv_bool_or_exception:
+  ∀ vs .
+    (∃ b . seqv vs = Val (SBool b)) ∨
+    (∃ s . seqv vs = Exception s)
+Proof
+  Cases
+  >> simp[seqv_def]
+  >> Cases_on ‘t’
+  >> simp[seqv_def]
+  >> Cases_on ‘t'’
+  >> simp[seqv_def]
+  >> IF_CASES_TAC
+  >> simp[]
+QED
+
+Theorem valid_state_progress:
+  ∀ store ks env state .
+    valid_state store ks env state
+    ⇒
+    ∃ store' ks' env' state' .
+      step (store, ks, env, state) = (store', ks', env', state') ∧
+      valid_state store' ks' env' state'
+Proof
+  Cases_on ‘state’
+  >> rpt strip_tac
+  >~ [‘Exp e’] >- (
+    Cases_on ‘e’
+    >~ [‘Lit l’] >- (
+      Cases_on ‘l’
+      >> simp[step_def, lit_to_val_def]
+      >> simp[Once valid_state_cases, Once valid_val_cases]
+      >> gvs[Once valid_state_cases]
+    )
+    >~ [‘Begin es e’] >- (
+      Cases_on ‘es’ >- (
+        simp[step_def, Once valid_state_cases]
+        >> gvs[Once valid_state_cases, Once static_scope_cases]
+      )
+      >> simp[step_def, Once valid_state_cases]
+      >> simp[Once valid_val_cases]
+      >> gvs[Once valid_state_cases, Once static_scope_cases]
+    )
+    >~ [‘Ident x’] >- (
+      simp[step_def]
+      >> gvs[Once valid_state_cases, Once static_scope_cases, can_lookup_cases]
+      >> ‘∀ x . FDOM env x ⇒ ∃ a. FLOOKUP env x = SOME a’
+        by simp[FLOOKUP_DEF, SPECIFICATION]
+      >> pop_assum drule >> strip_tac
+      >> drule_all_then assume_tac FEVERY_FLOOKUP
+      >> qpat_assum ‘EVERY _ _’ $ assume_tac o SRULE [EVERY_EL]
+      >> gvs[]
+      >> pop_assum $ drule_then assume_tac
+      >> ‘∀ x a . FLOOKUP env x = SOME a ⇒ env ' x = a’ by simp[FLOOKUP_DEF]
+      >> pop_assum $ drule_then assume_tac
+      >> simp[]
+      >> Cases_on ‘EL a store’ >- simp[Once valid_state_cases]
+      >> gvs[Once valid_state_cases, can_lookup_cases]
+    )
+    >~ [‘Letrec bs e’] >- (
+      simp[step_def]
+      >> rpt (pairarg_tac >> gvs[])
+      >> simp[Once valid_state_cases, Once static_scope_cases]
+      >> gvs[Once valid_state_cases, Once static_scope_cases]
+      >> drule_then assume_tac letrec_init_dom
+      >> drule_all_then assume_tac letrec_init_lookup
+      >> gvs[]
+      >> irule_at (Pos $ el 2) valid_cont_larger_store
+      >> qpat_assum ‘valid_cont _ _’ $ irule_at (Pos $ el 2)
+      >> simp[]
+      >> irule_at (Pos $ el 2) EVERY_MONOTONIC
+      >> qpat_assum ‘EVERY (OPTION_ALL _) _’ $ irule_at (Pos $ el 2)
+      >> strip_tac >- (
+        rpt strip_tac
+        >> irule_at (Pos hd) OPTION_ALL_MONO
+        >> pop_assum $ irule_at (Pos last)
+        >> rpt strip_tac
+        >> irule valid_val_larger_store
+        >> pop_assum $ irule_at (Pos last)
+        >> simp[]
+      )
+      >> simp[EVERY_GENLIST]
+      >> qpat_assum ‘EVERY _ (MAP SND bs)’ mp_tac
+      >> qpat_assum ‘FDOM _ ∪ _ = FDOM _’ mp_tac
+      >> rpt (pop_assum kall_tac)
+      >> qid_spec_tac ‘env’
+      >> Induct_on ‘bs’ >- simp[]
+      >> rpt strip_tac
+      >> PairCases_on ‘h’
+      >> simp[Once static_scope_cases]
+      >> gvs[]
+      >> last_x_assum $ qspec_then ‘env |+ (h0, 0)’ assume_tac
+      >> gvs[]
+      >> qsuff_tac ‘FDOM env ∪ (h0 INSERT set (MAP FST bs))
+        = (h0 INSERT FDOM env) ∪ set (MAP FST bs)’ >- (
+        strip_tac
+        >> pop_assum $ gvs o single
+        >> last_x_assum $ simp o single o GSYM
+      )
+      >> rpt $ pop_assum kall_tac
+      >> simp[EXTENSION, UNION_DEF]
+      >> strip_tac
+      >> iff_tac
+      >> strip_tac
+      >> simp[]
+    )
+    >> simp[step_def, Once valid_state_cases]
+    >> simp[Once valid_val_cases]
+    >> gvs[Once valid_state_cases, Once static_scope_cases, can_lookup_cases]
+  )
+  >~ [‘Val v’] >- (
+    Cases_on ‘ks’ >- (
+      simp[step_def, return_def, Once valid_state_cases,
+        can_lookup_cases, FEVERY_FEMPTY]
+      >> gvs[Once valid_state_cases]
+    )
+    >> PairCases_on ‘h’
+    >> Cases_on ‘h1’
+    >~ [‘CondK t f’] >- (
+      simp[step_def, return_def]
+      >> IF_CASES_TAC >- (
+        gvs[Once valid_state_cases, Once valid_val_cases]
+        >> gvs[Once valid_val_cases]
+        >> simp[Once valid_state_cases]
+      )
+      >> gvs[Once valid_state_cases]
+      >> qpat_x_assum ‘valid_cont _ _’ $ mp_tac o SRULE [Once valid_val_cases]
+      >> rpt strip_tac
+      >> simp[Once valid_state_cases]
+    )
+    >~ [‘BeginK es e’] >- (
+      simp[step_def, return_def]
+      >> CASE_TAC
+      >> gvs[Once valid_state_cases]
+      >> qpat_x_assum ‘valid_cont _ _’ $ mp_tac o SRULE [Once valid_val_cases]
+      >> rpt strip_tac
+      >> simp[Once valid_state_cases]
+      >> simp[Once valid_val_cases]
+    )
+    >~ [‘SetK x’] >- (
+      simp[step_def, return_def]
+      >> gvs[Once valid_state_cases]
+      >> qpat_x_assum ‘valid_cont _ _’ $ mp_tac o SRULE [Once valid_val_cases]
+      >> rpt strip_tac
+      >> simp[Once valid_state_cases]
+      >> simp[Once valid_val_cases]
+      >> irule_at (Pos hd) valid_cont_larger_store
+      >> qpat_assum ‘valid_cont _ _’ $ irule_at (Pos $ el 2)
+      >> simp[]
+      >> gvs[can_lookup_cases]
+      >> irule IMP_EVERY_LUPDATE
+      >> simp[OPTION_ALL_def]
+      >> irule_at (Pos hd) valid_val_larger_store
+      >> last_assum $ irule_at (Pos $ el 2)
+      >> simp[]
+      >> irule EVERY_MONOTONIC
+      >> qpat_assum ‘EVERY _ _’ $ irule_at (Pos last)
+      >> rpt strip_tac
+      >> irule OPTION_ALL_MONO
+      >> pop_assum $ irule_at (Pos last)
+      >> rpt strip_tac
+      >> irule_at (Pos hd) valid_val_larger_store
+      >> pop_assum $ irule_at (Pos last)
+      >> simp[]
+    )
+    >~ [‘ApplyK fnp es’] >- (
+      simp[step_def]
+      >> Cases_on ‘∃ e es' . es = e::es'’ >-(
+        gvs[]
+        >> Cases_on ‘∃ fn vs . fnp = SOME (fn,vs)’
+        >> Cases_on ‘fnp = NONE’
+        >> gvs[]
+        >> simp[return_def]
+        >> simp[Once valid_state_cases]
+        >> gvs[Once valid_state_cases]
+        >> simp[Once valid_val_cases]
+        >> qpat_x_assum ‘valid_cont _ _’ $ mp_tac o SRULE [Once valid_val_cases]
+        >> rpt strip_tac
+        >> simp[]
+        >> Cases_on ‘fnp’ >> gvs[] >> PairCases_on ‘x’ >> gvs[]
+      )
+      >> Cases_on ‘es’ >> gvs[]
+      >> Cases_on ‘fnp’ >- (
+        simp[return_def]
+        >> Cases_on ‘v’
+        >> simp[application_def]
+        >~ [‘Prim p’] >- (
+          CASE_TAC
+          >> simp[Once valid_state_cases, sadd_def, smul_def,
+            sminus_def, seqv_def, can_lookup_cases, FEVERY_FEMPTY]
+          >> simp[Once valid_val_cases]
+          >> gvs[Once valid_state_cases]
+          >> qpat_x_assum ‘valid_cont _ _’ $ mp_tac o SRULE [Once valid_val_cases]
+          >> simp[]
+        )
+        >~ [‘Proc env' xs xp e’] >- (
+          Cases_on ‘xp’
+          >> Cases_on ‘xs’
+          >> simp[parameterize_def] >- (
+            simp[Once valid_state_cases]
+            >> gvs[Once valid_state_cases]
+            >> gvs[Once valid_val_cases]
+            >> gvs[Once valid_val_cases]
+          )
+          >- simp[Once valid_state_cases]
+          >- (
+            rpt (pairarg_tac >> gvs[])
+            >> simp[Once valid_state_cases]
+            >> gvs[Once valid_state_cases, fresh_loc_def]
+            >> gvs[Once valid_val_cases]
+            >> gvs[Once valid_val_cases]
+            >> simp[Once INSERT_SING_UNION, Once UNION_COMM]
+            >> irule_at (Pos hd) valid_cont_larger_store
+            >> qpat_assum ‘valid_cont _ _’ $ irule_at (Pos $ el 2)
+            >> simp[Once valid_val_cases]
+            >> irule_at (Pos $ el 2) $ EVERY_MONOTONIC
+            >> pop_assum $ irule_at (Pos $ el 2)
+            >> gvs[can_lookup_cases]
+            >> irule_at (Pos $ el 2) $ cj 2 FEVERY_STRENGTHEN_THM
+            >> simp[]
+            >> irule_at (Pos hd) FEVERY_MONO
+            >> qpat_assum ‘FEVERY _ env'’ $ irule_at (Pos $ el 2)
+            >> rpt strip_tac >- (PairCases_on ‘x'’ >> gvs[])
+            >> irule OPTION_ALL_MONO
+            >> pop_assum $ irule_at (Pos last)
+            >> rpt strip_tac
+            >> irule valid_val_larger_store
+            >> pop_assum $ irule_at (Pos last)
+            >> simp[]
+          )
+          >> simp[Once valid_state_cases]
+          >> gvs[Once valid_state_cases]
+          >> gvs[Once valid_val_cases]
+          >> gvs[Once valid_val_cases]
+        )
+        >> simp[Once valid_state_cases]
+        >> gvs[Once valid_state_cases]
+        >> gvs[Once valid_val_cases]
+        >> gvs[Once valid_val_cases]
+      )
+      >> PairCases_on ‘x’
+      >> simp[return_def]
+      >> Cases_on ‘x0’
+      >> simp[application_def]
+      >~ [‘Prim p’] >- (
+        TOP_CASE_TAC >- (
+          qspecl_then [‘REVERSE x1 ++ [v]’, ‘0’] assume_tac sadd_num_or_exception
+          >> simp[Once valid_state_cases]
+          >> gvs[]
+          >> simp[Once valid_val_cases, can_lookup_cases, FEVERY_FEMPTY]
+          >> gvs[Once valid_state_cases]
+          >> qpat_x_assum ‘valid_cont _ _’ $ mp_tac o SRULE [Once valid_val_cases]
+          >> simp[]
+        )
+        >- (
+          qspecl_then [‘REVERSE x1 ++ [v]’, ‘1’] assume_tac smul_num_or_exception
+          >> simp[Once valid_state_cases]
+          >> gvs[]
+          >> simp[Once valid_val_cases, can_lookup_cases, FEVERY_FEMPTY]
+          >> gvs[Once valid_state_cases]
+          >> qpat_x_assum ‘valid_cont _ _’ $ mp_tac o SRULE [Once valid_val_cases]
+          >> simp[]
+        )
+        >- (
+          qspec_then ‘REVERSE x1 ++ [v]’ assume_tac sminus_num_or_exception
+          >> simp[Once valid_state_cases]
+          >> gvs[]
+          >> simp[Once valid_val_cases, can_lookup_cases, FEVERY_FEMPTY]
+          >> gvs[Once valid_state_cases]
+          >> qpat_x_assum ‘valid_cont _ _’ $ mp_tac o SRULE [Once valid_val_cases]
+          >> simp[]
+        )
+        >- (
+          qspec_then ‘REVERSE x1 ++ [v]’ assume_tac seqv_bool_or_exception
+          >> simp[Once valid_state_cases]
+          >> gvs[]
+          >> simp[Once valid_val_cases, can_lookup_cases, FEVERY_FEMPTY]
+          >> gvs[Once valid_state_cases]
+          >> qpat_x_assum ‘valid_cont _ _’ $ mp_tac o SRULE [Once valid_val_cases]
+          >> simp[]
+        )
+        >> CASE_TAC
+        >> gvs[]
+        >> Cases_on ‘t'’ >- (
+          gvs[]
+          >> simp[Once valid_state_cases]
+          >> gvs[Once valid_state_cases]
+          >> qpat_x_assum ‘valid_cont _ _’ $ mp_tac o SRULE [Once valid_val_cases]
+          >> rpt strip_tac
+          >> simp[Once valid_val_cases, can_lookup_cases, FEVERY_FEMPTY]
+        )
+        >> gvs[]
+        >> simp[Once valid_state_cases]
+        >> gvs[Once valid_state_cases]
+        >> gvs[Once valid_val_cases]
+        >> gvs[Once valid_val_cases]
+      )
+      >~ [‘Proc env' xs xp e’] >- (
+        rpt (pairarg_tac >> gvs[])
+        >> gvs[Once valid_state_cases]
+        >> qpat_x_assum ‘valid_cont _ _’ $ mp_tac o SRULE [Once valid_val_cases]
+        >> rpt strip_tac
+        >> qpat_x_assum ‘valid_val _ (Proc _ _ _ _)’ $ mp_tac o SRULE [Once valid_val_cases]
+        >> rpt strip_tac
+        >> gvs[] >- (
+          Cases_on ‘LENGTH xs = LENGTH (REVERSE x1 ++ [v])’ >- (
+            drule_all_then mp_tac parameterize_NONE_dom
+            >> drule_all_then mp_tac parameterize_NONE_lookup
+            >> rpt strip_tac
+            >> qpat_x_assum ‘Exp _ = _’ $ simp o single o GSYM
+            >> simp[Once valid_state_cases]
+            >> qpat_x_assum ‘_ ∪ _ = _’ $ simp o single o GSYM
+            >> qpat_x_assum ‘_ ++ _ = _’ $ simp o single o GSYM
+            >> irule_at (Pos hd) $ valid_cont_larger_store
+            >> qpat_assum ‘valid_cont _ _’ $ irule_at (Pos $ el 2)
+            >> simp[]
+            >> irule_at (Pos hd) EVERY_MONOTONIC
+            >> qpat_assum ‘EVERY _ store’ $ irule_at (Pos $ el 2)
+            >> strip_tac >- (
+              rpt strip_tac
+              >> irule OPTION_ALL_MONO
+              >> pop_assum $ irule_at (Pos last)
+              >> rpt strip_tac
+              >> irule valid_val_larger_store
+              >> pop_assum $ irule_at (Pos last)
+              >> simp[]
+            )
+            >> strip_tac >- (
+              irule EVERY_OPTION_ALL_MAP_SOME
+              >> irule EVERY_MONOTONIC
+              >> qexists ‘valid_val store’
+              >> simp[]
+              >> rpt strip_tac
+              >> irule valid_val_larger_store
+              >> pop_assum $ irule_at (Pos last)
+              >> simp[]
+            )
+            >> irule valid_val_larger_store
+            >> last_assum $ irule_at (Pos last)
+            >> simp[]
+          )
+          >> drule_all_then mp_tac parameterize_NONE_exception
+          >> rpt strip_tac
+          >> simp[Once valid_state_cases]
+          >> gvs[]
+        )
+        >> Cases_on ‘LENGTH xs ≤ LENGTH (REVERSE x1 ++ [v])’ >- (
+          drule_all_then mp_tac parameterize_SOME_dom
+          >> drule_all_then mp_tac parameterize_SOME_lookup
+          >> rpt strip_tac
+          >> simp[Once valid_state_cases]
+          >> gvs[]
+          >> irule_at (Pos hd) $ valid_cont_larger_store
+          >> qpat_assum ‘valid_cont _ _’ $ irule_at (Pos $ el 2)
+          >> simp[]
+          >> irule_at (Pos hd) EVERY_MONOTONIC
+          >> qpat_assum ‘EVERY _ store’ $ irule_at (Pos $ el 2)
+          >> strip_tac >- (
+            rpt strip_tac
+            >> irule OPTION_ALL_MONO
+            >> pop_assum $ irule_at (Pos last)
+            >> rpt strip_tac
+            >> irule valid_val_larger_store
+            >> pop_assum $ irule_at (Pos last)
+            >> simp[]
+          )
+          >> strip_tac >- (
+            irule EVERY_OPTION_ALL_MAP_SOME
+            >> irule EVERY_TAKE
+            >> simp[]
+            >> strip_tac >- (
+              irule EVERY_MONOTONIC
+              >> qpat_assum ‘EVERY _ x1’ $ irule_at (Pos last)
+              >> rpt strip_tac
+              >> irule valid_val_larger_store
+              >> pop_assum $ irule_at (Pos last)
+              >> simp[]
+            )
+            >> irule valid_val_larger_store
+            >> last_assum $ irule_at (Pos last)
+            >> simp[]
+          )
+          >> simp[Once valid_val_cases]
+          >> irule EVERY_TAKE
+          >> simp[]
+          >> strip_tac >- (
+            irule valid_val_larger_store
+            >> last_assum $ irule_at (Pos last)
+            >> simp[]
+          )
+          >> irule EVERY_MONOTONIC
+          >> qpat_assum ‘EVERY _ x1’ $ irule_at (Pos last)
+          >> rpt strip_tac
+          >> irule valid_val_larger_store
+          >> pop_assum $ irule_at (Pos last)
+          >> simp[]
+        )
+        >> ‘LENGTH (REVERSE x1 ++ [v]) < LENGTH xs’ by gvs[]
+        >> drule_all_then mp_tac parameterize_SOME_exception
+        >> rpt strip_tac
+        >> simp[Once valid_state_cases]
+        >> gvs[]
+      )
+      >~ [‘Throw ks’] >- (
+        CASE_TAC >- simp[Once valid_state_cases]
+        >> CASE_TAC >- (
+          gvs[]
+          >> simp[Once valid_state_cases, can_lookup_cases, FEVERY_FEMPTY]
+          >> gvs[Once valid_state_cases]
+          >> qpat_x_assum ‘valid_cont _ _’ $ mp_tac o SRULE [Once valid_val_cases]
+          >> rpt strip_tac
+          >> qpat_x_assum ‘valid_val _ _’ $ mp_tac o SRULE [Once valid_val_cases]
+          >> simp[]
+        )
+        >> simp[Once valid_state_cases]
+      )
+      >> simp[Once valid_state_cases]
+      >> gvs[Once valid_state_cases]
+      >> gvs[Once valid_val_cases]
+      >> gvs[Once valid_val_cases]
+    )
+  )
+  >> simp[step_def, Once valid_state_cases]
+QED
+
+Theorem statically_scoped_program_valid:
+  ∀ p . static_scope ∅ p ⇒ valid_state [] [] FEMPTY (Exp p)
+Proof
+  simp[Once valid_state_cases,
+    can_lookup_cases, FEVERY_FEMPTY]
+  >> simp[Once valid_val_cases]
+QED
 
 (*
   open scheme_semanticsTheory;
@@ -272,27 +1141,27 @@ End
     )
   ))] (Apply (Ident $ strlit "fac") [Val $ SNum 6]))”
 
-  EVAL “steps 500 ([], [], FEMPTY, Letrec [(strlit "fac", Lambda [strlit "x"] NONE (
-    Letrec [(strlit "st", Val $ SNum 0); (strlit "acc", Val $ SNum 1)] (
-      Begin ( Apply (Val $ Prim CallCC) [ Lambda [strlit "k"] NONE (
+  EVAL “steps 500 ([], [], FEMPTY, Exp $ Letrec [(strlit "fac", Lambda [strlit "x"] NONE (
+    Letrec [(strlit "st", Lit $ LitNum 0); (strlit "acc", Lit $ LitNum 1)] (
+      Begin [ Apply (Lit $ LitPrim CallCC) [ Lambda [strlit "k"] NONE (
         Set (strlit "st") (Ident $ strlit "k")
-      )]) [
-        Cond (Apply (Val $ Prim SEqv) [Ident $ strlit "x"; Val $ SNum 0])
+      )]] (
+        Cond (Apply (Lit $ LitPrim SEqv) [Ident $ strlit "x"; Lit $ LitNum 0])
           (Ident $ strlit "acc")
-          (Apply (Ident $ strlit "st") [ Begin (
-            Set (strlit "acc") (Apply (Val $ Prim SMul) [
+          (Apply (Ident $ strlit "st") [ Begin [
+            Set (strlit "acc") (Apply (Lit $ LitPrim SMul) [
               Ident $ strlit "acc";
               Ident $ strlit "x"
             ])
-          ) [
-            Set (strlit "x") (Apply (Val $ Prim SMinus) [
+          ] (
+            Set (strlit "x") (Apply (Lit $ LitPrim SMinus) [
               Ident $ strlit "x";
-              Val $ SNum 1
+              Lit $ LitNum 1
             ])
-          ]])
-      ]
+          )])
+      )
     )
-  ))] (Apply (Ident $ strlit "fac") [Val $ SNum 6]))”
+  ))] (Apply (Ident $ strlit "fac") [Lit $ LitNum 6]))”
 *)
 
 val _ = export_theory();
